first attempt to simplify FOL notations

theories/ordinals/Ackermann/LNN.v
@@ -23,7 +23,7 @@ Definition SysPrf := SysPrf LNN.
 #[local] Arguments atomic _ _ _ : clear implicits.
 
 Definition Plus (x y : Term) : Term :=
-  apply LNN Plus (Tcons x (Tcons y (Tnil))).
+  apply LNN Plus_ (Tcons x (Tcons y (Tnil))).
 
 Definition Times (x y : Term) : Term :=
   apply LNN Times (Tcons x (Tcons y (Tnil))).
@@ -48,11 +48,11 @@ Check zero.
 
 (* hidden by the next infixes ??? *)
  Notation "t1 + t2" := 
-  (apply  _ Languages.Plus 
+  (apply  _ Languages.Plus_ 
      (Tcons t1 (Tcons t2 (Tnil)))): 
     fol_scope.
 
-Notation "'Plus'' x  y" := (apply _ Languages.Plus (Tcons x (Tcons y (Tnil))))  (at level 50, x at level 0, left associativity): fol_scope.
+Notation "'Plus'' x  y" := (apply _ Languages.Plus_ (Tcons x (Tcons y (Tnil))))  (at level 50, x at level 0, left associativity): fol_scope.
 
 
 Notation "t1 * t2" := (apply  _ Languages.Times 
